BasicContextReduction.v
@@ -1,0 +1,198 @@
+(** * Context Reduction Basics *)
+
+(** Reformulation of de Boer and Bonsangue's basic setup in the context-reduction setting *)
+
+From Coq Require Import String Bool Datatypes Relations Program.Equality.
+From Coq Require Import Classes.RelationClasses.
+From Coq Require Import Logic.FunctionalExtensionality. (* for equality of substitutions *)
+
+From SymEx Require Import Expr.
+Import BasicExpr.
+
+From SymEx Require Import Maps.
+Import BasicMaps.
+
+From SymEx Require Import ContextReduction.
+
+Open Scope com_scope.
+
+Inductive Stmt : Type :=
+| SAsgn (x:string) (e:Aexpr)
+| SSeq (s1 s2:Stmt)
+| SIf (b:Bexpr) (s1 s2:Stmt)
+| SWhile (b:Bexpr) (s:Stmt)
+| SSkip.
+
+Notation "x := y"  :=
+         (SAsgn x y)
+            (in custom com at level 0, x constr at level 0,
+             y at level 85, no associativity) : com_scope.
+Notation "x ; y" :=
+         (SSeq x y)
+           (in custom com at level 90, right associativity) : com_scope.
+Notation "'if' x '{' y '}' '{' z '}'" :=
+         (SIf x y z)
+           (in custom com at level 89, x at level 99,
+            y at level 99, z at level 99) : com_scope.
+Notation "'while' x '{' y '}'" :=
+         (SWhile x y)
+           (in custom com at level 89, x at level 99,
+               y at level 99) : com_scope.
+Notation "'skip'" := SSkip (in custom com at level 80) : com_scope.
+
+Inductive is_context: (Stmt -> Stmt) -> Prop :=
+| is_context_hole: is_context (fun x => x)
+| is_context_seq: forall s C,
+    is_context C -> is_context (fun x => SSeq (C x) s).
+
+Inductive head_red__S: relation (sub * Bexpr * Stmt) :=
+| SAsgn_step: forall x e sig phi,
+    head_red__S (sig, phi, <{x := e}>) ((x !-> Aapply sig e; sig), phi, SSkip)
+| SIfTrue_step: forall b s1 s2 sig phi,
+    head_red__S (sig, phi, <{if b {s1} {s2}}>) (sig, BAnd phi (Bapply sig b), s1)
+| SIfFalse_step: forall b s1 s2 sig phi,
+    head_red__S (sig, phi, <{if b {s1} {s2}}>) (sig, BAnd phi (BNot (Bapply sig b)), s2)
+| SWhileTrue_step: forall b s sig phi,
+    head_red__S (sig, phi, <{while b {s}}>) (sig, BAnd phi (Bapply sig b), <{s ; while b {s}}>)
+| SWhileFalse_step: forall b s sig phi,
+    head_red__S (sig, phi, <{while b {s}}>) (sig, BAnd phi (BNot (Bapply sig b)), SSkip)
+| SSeq_skip: forall s sig phi,
+    head_red__S (sig, phi, <{skip ; s}>) (sig, phi, s)
+.
+
+Definition Sstep: relation (sub * Bexpr * Stmt) := context_red is_context head_red__S.
+Definition multi_Sstep := clos_refl_trans_n1 _ Sstep.
+
+Notation " c '->s' c'" := (Sstep c c') (at level 40).
+Notation " c '->*' c'" := (multi_Sstep c c') (at level 40).
+
+Inductive head_red__C: relation (Valuation * Stmt) :=
+| CAsgn_step: forall x e V,
+    head_red__C (V, <{x := e}>) ((x !-> Aeval V e ; V), SSkip)
+| CIfTrue_step: forall b s1 s2 V,
+    Beval V b = true ->
+    head_red__C (V, <{if b {s1} {s2}}>) (V, s1)
+| CIfFalse_step: forall b s1 s2 V,
+    Beval V b = false ->
+    head_red__C (V, <{if b {s1} {s2}}>) (V, s2)
+| CWhileTrue_step: forall b s V,
+    Beval V b = true ->
+    head_red__C (V, <{while b {s}}>) (V, <{s ; while b {s}}>)
+| CWhileFalse_step: forall b s V,
+    Beval V b = false ->
+    head_red__C (V, <{while b {s}}>) (V, SSkip)
+| CSeq_skip: forall s V,
+    head_red__C (V, <{skip ; s}>) (V, s)
+.
+
+Definition Cstep: relation (Valuation * Stmt) := context_red is_context head_red__C.
+Definition multi_Cstep := clos_refl_trans_n1 _ Cstep.
+
+Notation " c '=>c' c'" := (Cstep c c') (at level 40).
+Notation " c '=>*' c'" := (multi_Cstep c c') (at level 40).
+
+Theorem correctness : forall s s' sig phi V,
+    (id_sub, BTrue, s) ->* (sig, phi, s') ->
+    Beval V phi = true ->
+    (V, s) =>* (Comp V sig, s').
+Proof.
+  intros. dependent induction H.
+  - rewrite comp_id. constructor.
+  - dependent destruction H. destruct x as [sig0 phi0]. dependent destruction H; econstructor;
+    try (simpl in H2; apply andb_true_iff in H2; destruct H2; try (apply negb_true_iff in H2);
+      rewrite <- comp_subB in H2).
+    + constructor.
+      * rewrite asgn_sound. constructor.
+      * assumption.
+    + eapply IHclos_refl_trans_n1; try reflexivity; assumption.
+    + constructor.
+      * constructor. apply H2.
+      * assumption.
+    + eapply IHclos_refl_trans_n1; try reflexivity; assumption.
+    + constructor.
+      * apply CIfFalse_step. apply H2.
+      * assumption.
+    + eapply IHclos_refl_trans_n1; try reflexivity; assumption.
+    + constructor.
+      * apply CWhileTrue_step. apply H2.
+      * assumption.
+    + eapply IHclos_refl_trans_n1; try reflexivity; assumption.
+    + constructor.
+      * apply CWhileFalse_step. apply H2.
+      * assumption.
+    + eapply IHclos_refl_trans_n1; try reflexivity; assumption.
+    + constructor.
+      * apply CSeq_skip.
+      * assumption.
+    + eapply IHclos_refl_trans_n1; try reflexivity; assumption.
+Qed.
+
+Ltac splits := repeat (try split).
+
+Theorem completeness : forall s s' V0 V,
+    (V0, s) =>* (V, s') ->
+    exists sig phi, (id_sub, BTrue, s) ->* (sig, phi, s') /\ Beval V0 phi = true /\ V = Comp V0 sig.
+Proof.
+  intros. dependent induction H.
+  - exists id_sub. exists BTrue. splits. constructor.
+  - dependent destruction H. dependent destruction H.
+    + destruct (IHclos_refl_trans_n1 s (C <{x0 := e}>) V0 x) as [sig [phi [IHcomp [IHval IHupd]]]];
+        try reflexivity.
+      eexists. eexists. splits.
+      * econstructor.
+        ** constructor; [apply SAsgn_step
+                        | assumption].
+        ** apply IHcomp.
+      * assumption.
+      * rewrite asgn_sound. rewrite IHupd. reflexivity.
+    + destruct (IHclos_refl_trans_n1 s (C <{if b {s'0}{s2}}>) V0 V) as [sig [phi [IHcomp [IHval IHupd]]]];
+        try reflexivity.
+      eexists. eexists. splits.
+      * econstructor.
+        ** constructor; [apply SIfTrue_step
+                        | assumption].
+        ** apply IHcomp.
+      * simpl. apply andb_true_iff. split.
+        ** assumption.
+        ** rewrite <- comp_subB. rewrite <- IHupd. assumption.
+      * assumption.
+    + destruct (IHclos_refl_trans_n1 s (C <{if b {s1}{s'0}}>) V0 V) as [sig [phi [IHcomp [IHval IHupd]]]];
+        try reflexivity.
+      eexists. eexists. splits.
+      * econstructor.
+        ** constructor; [apply SIfFalse_step
+                        | assumption].
+        ** apply IHcomp.
+      * simpl. apply andb_true_iff. split.
+        ** assumption.
+        ** rewrite <- comp_subB. rewrite <- IHupd. apply negb_true_iff. assumption.
+      * assumption.
+    + destruct (IHclos_refl_trans_n1 s (C <{while b {s1}}>) V0 V) as [sig [phi [IHcomp [IHval IHupd]]]];
+        try reflexivity.
+      eexists. eexists. splits.
+      * econstructor.
+        ** constructor; [apply SWhileTrue_step
+                        | assumption].
+        ** apply IHcomp.
+      * simpl. apply andb_true_iff. split.
+        ** assumption.
+        ** rewrite <- comp_subB. rewrite <- IHupd. assumption.
+      * assumption.
+    + destruct (IHclos_refl_trans_n1 s (C <{while b {s1}}>) V0 V) as [sig [phi [IHcomp [IHval IHupd]]]];
+        try reflexivity.
+      eexists. eexists. splits.
+      * econstructor.
+        ** constructor; [apply SWhileFalse_step
+                        | assumption].
+        ** apply IHcomp.
+      * simpl. apply andb_true_iff. split.
+        ** assumption.
+        ** rewrite <- comp_subB. rewrite <- IHupd. apply negb_true_iff. assumption.
+      * assumption.
+    + destruct (IHclos_refl_trans_n1 s (C <{skip ; s'0}>) V0 V) as [sig [phi [IHcomp [IHval IHupd]]]];
+        try reflexivity.
+      exists sig. exists phi. splits; try assumption.
+      econstructor.
+      * constructor; [apply SSeq_skip | assumption].
+      *  apply IHcomp.
+Qed.
